version of ifc_def where the commands remaining to be executed are not compared in stack low-equivalence, not sure if this will be needed

ifc/ifc_no_cmd_inspection.v
@@ -22,7 +22,7 @@ Definition heap_clsf := heap_loc -> label.
 
 (* TODO this should match VST, i.e. we should have "state_pred = environ->mpred" for preconditions,
    and for postconditions, it's ret_assert in VST *)
-Definition state_pred := corestate -> mem -> Prop.
+Definition state_pred := env -> temp_env -> mem -> Prop.
 
 Definition pre_assert := environ -> mpred.
 (* "ret_assert := exitkind -> option val -> environ -> mpred" is already defined by VST *)
@@ -50,9 +50,16 @@ Definition gen_lo_equiv{Loc V: Type}(f1 f2: Loc -> label)(s1 s2: Loc -> V) :=
 Definition stack_lo_equiv(s1 s2: corestate)(N1 N2: stack_clsf): Prop :=
   match s1, s2 with
   | (State e1 te1 c1), (State e2 te2 c2) =>
-     e1 = e2 /\ c1 = c2 /\ gen_lo_equiv N1 N2 (fun i => te1 ! i) (fun i => te2 ! i)
+     e1 = e2 /\ gen_lo_equiv N1 N2 (fun i => te1 ! i) (fun i => te2 ! i)
   | _, _ => False
   end.
+
+Lemma stack_lo_equiv_change_cmd: forall e1 te1 c1 e2 te2 c2 c1' c2' N1 N2,
+  stack_lo_equiv (State e1 te1 c1 ) (State e2 te2 c2 ) N1 N2 ->
+  stack_lo_equiv (State e1 te1 c1') (State e2 te2 c2') N1 N2.
+Proof.
+  intros. unfold stack_lo_equiv in *. assumption.
+Qed.
 
 Definition heap_access(m: mem)(l: heap_loc): memval :=
   let (b, i) := l in (ZMap.get i (PMap.get b (Mem.mem_contents m))).
@@ -66,10 +73,10 @@ Definition simple_ifc {A : Type} (Delta: tycontext)
   (postP: A -> state_pred) (postN: A -> stack_clsf) (postA: A -> heap_clsf)
 := forall (x1 x2: A) (ge: genv) (e1 e2: env) (te1 te2: temp_env) (s1' s2': corestate)
           (m1 m1' m2 m2': mem) (n: nat),
+   preP x1 e1 te1 m1 ->
+   preP x2 e2 te2 m2 ->
    let s1 := (State e1 te1 [Kseq c]) in
    let s2 := (State e2 te2 [Kseq c]) in
-   preP x1 s1 m1 ->
-   preP x2 s2 m2 ->
    stack_lo_equiv s1 s2 (preN x1) (preN x2) ->
    heap_lo_equiv  m1 m2 (preA x1) (preA x2) ->
    star ge s1 m1 n s1' m1' ->
